Fix names

RegexCorrectness/NFA/Transition/Path/Basic.lean
@@ -77,38 +77,38 @@ theorem stepIn.nil_of_snoc {start} (h : stepIn nfa start i j (cs ++ [c])) :
 
 -- Idea: what if we require at least one step? (Making this a non-reflexive transitive closure)
 -- TODO: expand the motivation
-inductive pathIn' (nfa : NFA) (lowerBound : Nat) : (first : Nat) → (last : Nat) → (cs : List Char) → Prop where
-  | last (step : nfa.stepIn lowerBound i j cs) : nfa.pathIn' lowerBound i j cs
+inductive pathIn (nfa : NFA) (lowerBound : Nat) : (first : Nat) → (last : Nat) → (cs : List Char) → Prop where
+  | last (step : nfa.stepIn lowerBound i j cs) : nfa.pathIn lowerBound i j cs
   | more {i j k : Nat} {cs₁ cs₂ : List Char}
-    (step : nfa.stepIn lowerBound i j cs₁) (rest : nfa.pathIn' lowerBound j k cs₂) : nfa.pathIn' lowerBound i k (cs₁ ++ cs₂)
+    (step : nfa.stepIn lowerBound i j cs₁) (rest : nfa.pathIn lowerBound j k cs₂) : nfa.pathIn lowerBound i k (cs₁ ++ cs₂)
 
-theorem pathIn'.le_left (path : pathIn' nfa lb i j cs) : lb ≤ i := by
+theorem pathIn.le_left (path : pathIn nfa lb i j cs) : lb ≤ i := by
   cases path with
   | last step => exact step.h₁
   | more step => exact step.h₁
 
-theorem pathIn'.lt_left (path : pathIn' nfa lb i j cs) : i < nfa.nodes.size := by
+theorem pathIn.lt_left (path : pathIn nfa lb i j cs) : i < nfa.nodes.size := by
   cases path with
   | last step => exact step.h₂
   | more step => exact step.h₂
 
-theorem pathIn'.lt_right (path : pathIn' nfa lb i j cs) : j < nfa.nodes.size := by
+theorem pathIn.lt_right (path : pathIn nfa lb i j cs) : j < nfa.nodes.size := by
   induction path with
   | last step => exact step.lt_right
   | more _ _ ih => exact ih
 
-theorem pathIn'.castBound {nfa : NFA} {lb lb' : Nat}
+theorem pathIn.castBound {nfa : NFA} {lb lb' : Nat}
   (le : lb' ≤ lb)
-  (path : nfa.pathIn' lb i j cs) :
-  nfa.pathIn' lb' i j cs := by
+  (path : nfa.pathIn lb i j cs) :
+  nfa.pathIn lb' i j cs := by
   induction path with
   | last step => exact .last (step.castStart le)
   | more step _ ih => exact .more (step.castStart le) ih
 
-theorem pathIn'.cast {nfa nfa' : NFA} (lb : Nat)
+theorem pathIn.cast {nfa nfa' : NFA} (lb : Nat)
   (eq : ∀ i, (h₁ : lb ≤ i) → (h₂ : i < nfa.nodes.size) → ∃ h' : i < nfa'.nodes.size, nfa[i] = nfa'[i])
-  (path : pathIn' nfa lb i j cs) :
-  pathIn' nfa' lb i j cs := by
+  (path : pathIn nfa lb i j cs) :
+  pathIn nfa' lb i j cs := by
   induction path with
   | last step =>
     have ⟨isLt, eq⟩ := eq _ step.h₁ step.h₂
@@ -117,11 +117,11 @@ theorem pathIn'.cast {nfa nfa' : NFA} (lb : Nat)
     have ⟨isLt, eq⟩ := eq _ step.h₁ step.h₂
     exact .more (step.cast isLt eq) ih
 
-theorem pathIn'.cast' {nfa nfa' : NFA} {lb : Nat}
+theorem pathIn.cast' {nfa nfa' : NFA} {lb : Nat}
   (assm : i < nfa.nodes.size) (le : nfa.nodes.size ≤ nfa'.nodes.size)
   (eq : ∀ i, (h₁ : lb ≤ i) → (h₂ : i < nfa.nodes.size) → nfa[i] = nfa'[i]'(Nat.lt_of_lt_of_le h₂ le))
-  (path : pathIn' nfa' lb i j cs) :
-  pathIn' nfa lb i j cs := by
+  (path : pathIn nfa' lb i j cs) :
+  pathIn nfa lb i j cs := by
   induction path with
   | last step => exact .last (step.cast assm (eq _ step.h₁ assm).symm)
   | more step _ ih =>
@@ -129,15 +129,15 @@ theorem pathIn'.cast' {nfa nfa' : NFA} {lb : Nat}
     have rest := ih step'.lt_right
     exact .more step' rest
 
-theorem pathIn'.castLE {nfa : NFA} {lb lb' i i' : Nat}
+theorem pathIn.castLE {nfa : NFA} {lb lb' i i' : Nat}
   (assm : lb' ≤ i)
   (inBounds : ∀ i j, (h₁ : lb' ≤ i) →
     (h₂ : i < nfa.nodes.size) →
     (∃ c, j ∈ nfa[i].charStep c) ∨ j ∈ nfa[i].εStep →
     lb ≤ j →
     lb' ≤ j)
-  (path : pathIn' nfa lb i i' cs) :
-  pathIn' nfa lb' i i' cs := by
+  (path : pathIn nfa lb i i' cs) :
+  pathIn nfa lb' i i' cs := by
   induction path with
   | last step => exact .last (step.castStart' assm)
   | @more i j k cs₁ cs₂ step rest ih =>
@@ -149,9 +149,9 @@ theorem pathIn'.castLE {nfa : NFA} {lb lb' i i' : Nat}
     have rest' := ih this
     exact .more step' rest'
 
-theorem pathIn'.snoc_char (path : pathIn' nfa lb i j cs) (assm : min lb k ≤ j)
+theorem pathIn.snoc_char (path : pathIn nfa lb i j cs) (assm : min lb k ≤ j)
   (step : k ∈ (nfa[j]'path.lt_right).charStep c)
-  : pathIn' nfa (min lb k) i k (cs ++ [c]) := by
+  : pathIn nfa (min lb k) i k (cs ++ [c]) := by
   induction path with
   | @last i j cs step' =>
     have step'' : nfa.stepIn (min lb k) j k [c] := .charStep assm step'.lt_right step
@@ -160,12 +160,12 @@ theorem pathIn'.snoc_char (path : pathIn' nfa lb i j cs) (assm : min lb k ≤ j)
     simp
     exact .more (step'.castStart (Nat.min_le_left _ _)) (ih assm step)
 
-theorem pathIn'.snoc_ε (path : pathIn' nfa lb i j cs) (assm : min lb k ≤ j)
+theorem pathIn.snoc_ε (path : pathIn nfa lb i j cs) (assm : min lb k ≤ j)
   (step : k ∈ (nfa[j]'path.lt_right).εStep)
-  : pathIn' nfa (min lb k) i k cs := by
+  : pathIn nfa (min lb k) i k cs := by
   induction path with
   | @last i j cs step' =>
-    suffices nfa.pathIn' (min lb k) i k (cs ++ []) by
+    suffices nfa.pathIn (min lb k) i k (cs ++ []) by
       simp at this
       exact this
     have step'' : nfa.stepIn (min lb k) j k [] := .εStep assm step'.lt_right step
@@ -173,8 +173,8 @@ theorem pathIn'.snoc_ε (path : pathIn' nfa lb i j cs) (assm : min lb k ≤ j)
   | @more i j k cs₁ cs₂ step' _ ih =>
     exact .more (step'.castStart (Nat.min_le_left _ _)) (ih assm step)
 
-theorem pathIn'.trans (path₁ : pathIn' nfa lb i j cs) (path₂ : pathIn' nfa lb j k cs') :
-  pathIn' nfa lb i k (cs ++ cs') := by
+theorem pathIn.trans (path₁ : pathIn nfa lb i j cs) (path₂ : pathIn nfa lb j k cs') :
+  pathIn nfa lb i k (cs ++ cs') := by
   induction path₁ with
   | last step => exact .more step path₂
   | more step _ ih =>
