RegexCorrectness/NFA/Transition/Closure/Equivalence.lean
@@ -5,7 +5,7 @@ import Mathlib.Data.List.Indexes
 
 namespace Regex.NFA
 
-theorem εClosure_of_pathIn' {nfa : NFA} (path : nfa.pathIn' lb i i' []) :
+theorem εClosure_of_pathIn {nfa : NFA} (path : nfa.pathIn lb i i' []) :
   i' ∈ nfa.εClosure i := by
   generalize h : [] = cs at path
   induction path with
@@ -20,8 +20,8 @@ theorem εClosure_of_pathIn' {nfa : NFA} (path : nfa.pathIn' lb i i' []) :
     | εStep _ _ step =>
       exact εClosure.step (εStep_of_εStep step) ih
 
-theorem eq_or_pathIn'_of_εClosure {nfa : NFA} (cls : i' ∈ nfa.εClosure i) :
-  i = i' ∨ nfa.pathIn' 0 i i' [] := by
+theorem eq_or_pathIn_of_εClosure {nfa : NFA} (cls : i' ∈ nfa.εClosure i) :
+  i = i' ∨ nfa.pathIn 0 i i' [] := by
   induction cls with
   | base => exact .inl rfl
   | @step i j k step rest ih =>
@@ -37,11 +37,11 @@ theorem eq_or_pathIn'_of_εClosure {nfa : NFA} (cls : i' ∈ nfa.εClosure i) :
       | isFalse nlt => simp [εStep, nlt] at step
 
 -- TODO: explain
-theorem pathIn'.of_snoc_char (assm : cs' = cs ++ [c])
-  (path : pathIn' nfa lb i l cs') :
+theorem pathIn.of_snoc_char (assm : cs' = cs ++ [c])
+  (path : pathIn nfa lb i l cs') :
   ∃ j k,
-    (nfa.stepIn lb i k cs' ∨ (nfa.pathIn' lb i j cs ∧ nfa.stepIn lb j k [c])) ∧
-    (k = l ∨ nfa.pathIn' lb k l []) := by
+    (nfa.stepIn lb i k cs' ∨ (nfa.pathIn lb i j cs ∧ nfa.stepIn lb j k [c])) ∧
+    (k = l ∨ nfa.pathIn lb k l []) := by
   induction path generalizing cs with
   | @last i j cs' step =>
     cases step with
@@ -86,12 +86,12 @@ where
         exact ⟨h₁.left, h₂⟩
       simp [this]
 
-theorem eq_or_pathIn'_of_reaches {nfa : NFA} {i : Fin nfa.nodes.size} {m : List Char}
+theorem eq_or_pathIn_of_reaches {nfa : NFA} {i : Fin nfa.nodes.size} {m : List Char}
   (h : nfa.reaches i m) :
-  (nfa.start = i ∧ m = []) ∨ nfa.pathIn' 0 nfa.start i m := by
+  (nfa.start = i ∧ m = []) ∨ nfa.pathIn 0 nfa.start i m := by
   induction h with
   | nil cls =>
-    cases eq_or_pathIn'_of_εClosure cls with
+    cases eq_or_pathIn_of_εClosure cls with
     | inl eq => exact .inl ⟨Fin.eq_of_val_eq eq, rfl⟩
     | inr path => exact .inr path
   | @snoc i j k c m _ step cls ih =>
@@ -99,13 +99,13 @@ theorem eq_or_pathIn'_of_reaches {nfa : NFA} {i : Fin nfa.nodes.size} {m : List 
     cases ih with
     | inl eq =>
       simp [eq]
-      cases eq_or_pathIn'_of_εClosure cls with
+      cases eq_or_pathIn_of_εClosure cls with
       | inl eq => exact .last (.charStep (Nat.zero_le _) i.isLt (eq ▸ step))
       | inr path => exact .more (.charStep (Nat.zero_le _) i.isLt step) path
     | inr path =>
       have := path.snoc_char (by simp) step
       simp at this
-      cases eq_or_pathIn'_of_εClosure cls with
+      cases eq_or_pathIn_of_εClosure cls with
       | inl eq =>
         rw [eq] at this
         exact .inr this
@@ -114,17 +114,17 @@ theorem eq_or_pathIn'_of_reaches {nfa : NFA} {i : Fin nfa.nodes.size} {m : List 
         simp at this
         exact .inr this
 
-theorem reaches_of_pathIn' {nfa : NFA} {i : Fin nfa.nodes.size} {m : List Char}
-  (h : nfa.pathIn' 0 nfa.start i m) :
+theorem reaches_of_pathIn {nfa : NFA} {i : Fin nfa.nodes.size} {m : List Char}
+  (h : nfa.pathIn 0 nfa.start i m) :
   nfa.reaches i m := by
   induction m using List.list_reverse_induction generalizing i with
-  | base => exact .nil (εClosure_of_pathIn' h)
+  | base => exact .nil (εClosure_of_pathIn h)
   | ind m c ih =>
-    have ⟨j, k, h₁, h₂⟩ := pathIn'.of_snoc_char rfl h
+    have ⟨j, k, h₁, h₂⟩ := pathIn.of_snoc_char rfl h
     have cls : i.val ∈ nfa.εClosure k := by
       cases h₂ with
       | inl eq => exact eq ▸ .base
-      | inr path => exact εClosure_of_pathIn' path
+      | inr path => exact εClosure_of_pathIn path
     match h₁ with
     | .inl step =>
       have := step.nil_of_snoc
@@ -136,11 +136,11 @@ theorem reaches_of_pathIn' {nfa : NFA} {i : Fin nfa.nodes.size} {m : List Char}
       cases step with
       | charStep _ _ step => exact .snoc prev (charStep_of_charStep step) cls
 
-theorem matches_of_reaches' (eq : compile r = nfa)
+theorem matches_of_reaches (eq : compile r = nfa)
   (h₁ : nfa.reaches i cs) (h₂ : nfa[i] = .done) :
   r.matches cs := by
   have hi : i.val = 0 := (done_iff_zero_compile eq i).mp h₂
-  have path := eq_or_pathIn'_of_reaches h₁
+  have path := eq_or_pathIn_of_reaches h₁
   have : nfa.start ≠ i := by
     apply Fin.ne_of_val_ne
     rw [hi]
@@ -150,19 +150,19 @@ theorem matches_of_reaches' (eq : compile r = nfa)
     rw [←eq]
     exact ge_pushRegex_start h
   simp [this] at path
-  exact (matches_iff_pathIn' eq).mpr (hi ▸ path)
+  exact (matches_iff_pathIn eq).mpr (hi ▸ path)
 
-theorem reaches_of_matches' (eq : compile r = nfa)
+theorem reaches_of_matches (eq : compile r = nfa)
   (m : r.matches cs) :
   ∃ i, nfa.reaches i cs ∧ nfa[i] = .done := by
-  have := (matches_iff_pathIn' eq).mp m
+  have := (matches_iff_pathIn eq).mp m
   let i' : Fin nfa.nodes.size := ⟨0, lt_zero_size_compile eq⟩
-  have := reaches_of_pathIn' (i := i') this
+  have := reaches_of_pathIn (i := i') this
   have hdone := (done_iff_zero_compile eq i').mpr rfl
   exact ⟨i', this, hdone⟩
 
 theorem matches_iff_reaches (eq : compile r = nfa) :
   r.matches cs ↔ ∃ i, nfa.reaches i cs ∧ nfa[i] = .done :=
-  ⟨reaches_of_matches' eq, fun ⟨_, h₁, h₂⟩ => matches_of_reaches' eq h₁ h₂⟩
+  ⟨reaches_of_matches eq, fun ⟨_, h₁, h₂⟩ => matches_of_reaches eq h₁ h₂⟩
 
 end Regex.NFA
