RegexCorrectness/NFA/Transition/Path/Equivalence/PathOfMatch.lean
@@ -11,35 +11,35 @@ namespace Regex.NFA
 theorem pathIn_of_matches.group {cs : List Char}
   (eq : pushRegex nfa next (.group i r) = nfa')
   (ih : ∀ {nfa next nfa'}, pushRegex nfa next r = nfa' →
-    pathIn' nfa' nfa.nodes.size nfa'.val.start next cs) :
-  pathIn' nfa' nfa.nodes.size nfa'.val.start next cs := by
+    pathIn nfa' nfa.nodes.size nfa'.val.start next cs) :
+  pathIn nfa' nfa.nodes.size nfa'.val.start next cs := by
   apply pushRegex.group eq
   intro nfa' nfa'' nfa''' property _ _ eq₁ eq₂ eq₃ eq
   rw [eq]
   simp
-  have path₃ : pathIn' nfa' nfa.nodes.size nfa'.val.start next [] := by
+  have path₃ : pathIn nfa' nfa.nodes.size nfa'.val.start next [] := by
     have h₁ : nfa.nodes.size ≤ nfa'.val.start.val := by
       rw [eq₁]
       simp
     refine .last (.εStep h₁ nfa'.val.start.isLt ?_)
     rw [eq₁]
     simp [Node.εStep]
-  have path₃ : pathIn' nfa'' nfa.nodes.size nfa'.val.start next [] := by
+  have path₃ : pathIn nfa'' nfa.nodes.size nfa'.val.start next [] := by
     apply path₃.cast
     intro i _ h₂
     exists Nat.lt_trans h₂ nfa''.property
     rw [pushRegex_get_lt eq₂.symm _ h₂]
-  have path₂ : pathIn' nfa'' nfa'.val.nodes.size nfa''.val.start nfa'.val.start cs :=
+  have path₂ : pathIn nfa'' nfa'.val.nodes.size nfa''.val.start nfa'.val.start cs :=
     ih eq₂.symm
-  have path₂₃ : pathIn' nfa'' nfa.nodes.size nfa''.val.start next (cs ++ []) :=
-    pathIn'.trans (path₂.castBound (Nat.le_of_lt nfa'.property)) path₃
+  have path₂₃ : pathIn nfa'' nfa.nodes.size nfa''.val.start next (cs ++ []) :=
+    pathIn.trans (path₂.castBound (Nat.le_of_lt nfa'.property)) path₃
   simp at path₂₃
-  have path₂₃ : pathIn' nfa''' nfa.nodes.size nfa''.val.start next cs := by
+  have path₂₃ : pathIn nfa''' nfa.nodes.size nfa''.val.start next cs := by
     apply path₂₃.cast
     intro i _ h₂
     exists Nat.lt_trans h₂ nfa'''.property
     rw [eq₃, pushNode_get_lt _ h₂]
-  have path₁ : pathIn' nfa''' nfa.nodes.size nfa'''.val.start nfa''.val.start [] := by
+  have path₁ : pathIn nfa''' nfa.nodes.size nfa'''.val.start nfa''.val.start [] := by
     have h₁ : nfa.nodes.size ≤ nfa'''.val.start.val := by
       rw [eq₃]
       simp
@@ -52,14 +52,14 @@ theorem pathIn_of_matches.group {cs : List Char}
 theorem pathIn_of_matches.alternateLeft {cs : List Char}
   (eq : pushRegex nfa next (.alternate r₁ r₂) = nfa')
   (ih : ∀ {nfa next nfa'}, pushRegex nfa next r₁ = nfa' →
-    pathIn' nfa' nfa.nodes.size nfa'.val.start next cs) :
-  pathIn' nfa' nfa.nodes.size nfa'.val.start next cs := by
+    pathIn nfa' nfa.nodes.size nfa'.val.start next cs) :
+  pathIn nfa' nfa.nodes.size nfa'.val.start next cs := by
   apply pushRegex.alternate eq
   intro nfa₁ start₁ nfa₂ start₂ _ nfa' property eq₁ eq₂ eq₃ _ eq₅ eq
   rw [eq]
   simp
-  have : pathIn' nfa₁ nfa.nodes.size nfa₁.val.start next cs := ih eq₁.symm
-  have : pathIn' nfa' nfa.nodes.size nfa₁.val.start next cs := by
+  have : pathIn nfa₁ nfa.nodes.size nfa₁.val.start next cs := ih eq₁.symm
+  have : pathIn nfa' nfa.nodes.size nfa₁.val.start next cs := by
     apply this.cast
     intro i _ h₂
     have lt₂ : i < nfa₂.val.nodes.size := Nat.lt_trans h₂ nfa₂.property
@@ -68,7 +68,7 @@ theorem pathIn_of_matches.alternateLeft {cs : List Char}
     simp [eq₅]
     rw [pushNode_get_lt _ lt₂]
     rw [pushRegex_get_lt eq₃.symm _ h₂]
-  have : pathIn' nfa' nfa.nodes.size nfa'.val.start next ([] ++ cs) := by
+  have : pathIn nfa' nfa.nodes.size nfa'.val.start next ([] ++ cs) := by
     refine .more (.εStep ?_ nfa'.val.start.isLt ?_) this
     . rw [eq₅]
       simp
@@ -81,22 +81,22 @@ theorem pathIn_of_matches.alternateLeft {cs : List Char}
 theorem pathIn_of_matches.alternateRight {cs : List Char}
   (eq : pushRegex nfa next (.alternate r₁ r₂) = nfa')
   (ih : ∀ {nfa next nfa'}, pushRegex nfa next r₂ = nfa' →
-    pathIn' nfa' nfa.nodes.size nfa'.val.start next cs) :
-  pathIn' nfa' nfa.nodes.size nfa'.val.start next cs := by
+    pathIn nfa' nfa.nodes.size nfa'.val.start next cs) :
+  pathIn nfa' nfa.nodes.size nfa'.val.start next cs := by
   apply pushRegex.alternate eq
   intro nfa₁ start₁ nfa₂ start₂ _ nfa' property _ _ eq₃ eq₄ eq₅ eq
   rw [eq]
   simp
-  have : pathIn' nfa₂ nfa.nodes.size nfa₂.val.start next cs :=
+  have : pathIn nfa₂ nfa.nodes.size nfa₂.val.start next cs :=
     (ih eq₃.symm).castBound (Nat.le_of_lt nfa₁.property)
-  have : pathIn' nfa' nfa.nodes.size nfa₂.val.start next cs := by
+  have : pathIn nfa' nfa.nodes.size nfa₂.val.start next cs := by
     apply this.cast
     intro i _ h₂
     have : i < nfa'.val.nodes.size := Nat.lt_trans h₂ nfa'.property
     exists this
     simp [eq₅]
     rw [pushNode_get_lt _ h₂]
-  have : pathIn' nfa' nfa.nodes.size nfa'.val.start next ([] ++ cs) := by
+  have : pathIn nfa' nfa.nodes.size nfa'.val.start next ([] ++ cs) := by
     refine .more (.εStep ?_ nfa'.val.start.isLt ?_) this
     . rw [eq₅]
       simp
@@ -109,18 +109,18 @@ theorem pathIn_of_matches.alternateRight {cs : List Char}
 theorem pathIn_of_matches.concat {cs₁ cs₂ : List Char}
   (eq : pushRegex nfa next (.concat r₁ r₂) = nfa')
   (ih₁ : ∀ {nfa next nfa'}, pushRegex nfa next r₁ = nfa' →
-    pathIn' nfa' nfa.nodes.size nfa'.val.start next cs₁)
+    pathIn nfa' nfa.nodes.size nfa'.val.start next cs₁)
   (ih₂ : ∀ {nfa next nfa'}, pushRegex nfa next r₂ = nfa' →
-    pathIn' nfa' nfa.nodes.size nfa'.val.start next cs₂) :
-  pathIn' nfa' nfa.nodes.size nfa'.val.start next (cs₁ ++ cs₂) := by
+    pathIn nfa' nfa.nodes.size nfa'.val.start next cs₂) :
+  pathIn nfa' nfa.nodes.size nfa'.val.start next (cs₁ ++ cs₂) := by
   apply pushRegex.concat eq
   intro nfa₂ nfa₁ property eq₂ eq₁ eq
   rw [eq]
   simp
-  have ih₁ : pathIn' nfa₁ nfa.nodes.size nfa₁.val.start nfa₂.val.start cs₁ :=
+  have ih₁ : pathIn nfa₁ nfa.nodes.size nfa₁.val.start nfa₂.val.start cs₁ :=
     (ih₁ eq₁.symm).castBound (Nat.le_of_lt nfa₂.property)
-  have ih₂ : pathIn' nfa₂ nfa.nodes.size nfa₂.val.start next cs₂ := ih₂ eq₂.symm
-  have ih₂ : pathIn' nfa₁ nfa.nodes.size nfa₂.val.start next cs₂ := by
+  have ih₂ : pathIn nfa₂ nfa.nodes.size nfa₂.val.start next cs₂ := ih₂ eq₂.symm
+  have ih₂ : pathIn nfa₁ nfa.nodes.size nfa₂.val.start next cs₂ := by
     apply ih₂.cast
     intro i _ h₂
     exists Nat.lt_trans h₂ nfa₁.property
@@ -130,11 +130,11 @@ theorem pathIn_of_matches.concat {cs₁ cs₂ : List Char}
 theorem pathIn_of_matches.starConcat {cs₁ cs₂ : List Char}
   (eq : pushRegex nfa next (.star r) = nfa')
   (ih₁ : ∀ {nfa next nfa'}, pushRegex nfa next r = nfa' →
-    pathIn' nfa' nfa.nodes.size nfa'.val.start next cs₁)
+    pathIn nfa' nfa.nodes.size nfa'.val.start next cs₁)
   (ih₂ : ∀ {nfa next nfa'}, pushRegex nfa next (.star r) = nfa' →
-    pathIn' nfa' nfa.nodes.size nfa'.val.start next cs₂) :
-  pathIn' nfa' nfa.nodes.size nfa'.val.start next (cs₁ ++ cs₂) := by
-  have ih₂ : pathIn' nfa' nfa.nodes.size nfa'.val.start next cs₂ := ih₂ eq
+    pathIn nfa' nfa.nodes.size nfa'.val.start next cs₂) :
+  pathIn nfa' nfa.nodes.size nfa'.val.start next (cs₁ ++ cs₂) := by
+  have ih₂ : pathIn nfa' nfa.nodes.size nfa'.val.start next cs₂ := ih₂ eq
   apply pushRegex.star eq
   intro placeholder compiled patched nfa' isLt inBounds property
     eq₁ eq₂ eq₃ eq₄ eq
@@ -144,9 +144,9 @@ theorem pathIn_of_matches.starConcat {cs₁ cs₂ : List Char}
   simp at ih₂
   have eqStart : nfa'.start = nfa.nodes.size := by
     rw [eq₄]
-  have ih₁ : pathIn' compiled placeholder.val.nodes.size compiled.val.start nfa.nodes.size cs₁ :=
+  have ih₁ : pathIn compiled placeholder.val.nodes.size compiled.val.start nfa.nodes.size cs₁ :=
     ih₁ eq₂.symm
-  have ih₁ : pathIn' nfa' placeholder.val.nodes.size compiled.val.start nfa.nodes.size cs₁ := by
+  have ih₁ : pathIn nfa' placeholder.val.nodes.size compiled.val.start nfa.nodes.size cs₁ := by
     apply ih₁.cast
     intro i h₁ h₂
     rw [eq₄]
@@ -156,13 +156,13 @@ theorem pathIn_of_matches.starConcat {cs₁ cs₂ : List Char}
     rw [Array.get_set_ne (hj := h₂)]
     simp
     apply Nat.ne_of_lt (Nat.lt_of_lt_of_le placeholder.property h₁)
-  have ih₁ : pathIn' nfa' nfa.nodes.size compiled.val.start nfa.nodes.size cs₁ :=
+  have ih₁ : pathIn nfa' nfa.nodes.size compiled.val.start nfa.nodes.size cs₁ :=
     ih₁.castBound (Nat.le_of_lt placeholder.property)
-  have ih₂ : pathIn' nfa' nfa.nodes.size nfa.nodes.size next cs₂ := by
+  have ih₂ : pathIn nfa' nfa.nodes.size nfa.nodes.size next cs₂ := by
     rw [eqStart] at ih₂
     exact ih₂
   have := ih₁.trans ih₂
-  have : pathIn' nfa' nfa.nodes.size nfa'.start next ([] ++ (cs₁ ++ cs₂)) := by
+  have : pathIn nfa' nfa.nodes.size nfa'.start next ([] ++ (cs₁ ++ cs₂)) := by
     refine .more (.εStep (by simp [eqStart]) nfa'.start.isLt ?_) this
     rw [eq₄]
     simp [get_eq_nodes_get, eq₃, Node.εStep]
@@ -171,7 +171,7 @@ theorem pathIn_of_matches.starConcat {cs₁ cs₂ : List Char}
 
 theorem pathIn_of_matches (eq : pushRegex nfa next r = nfa')
   (m : r.matches cs) :
-  pathIn' nfa' nfa.nodes.size nfa'.val.start next cs := by
+  pathIn nfa' nfa.nodes.size nfa'.val.start next cs := by
   induction m generalizing nfa next with
   | char c =>
     have : nfa.nodes.size ≤ nfa'.val.start.val := ge_pushRegex_start eq
@@ -208,7 +208,7 @@ theorem pathIn_of_matches (eq : pushRegex nfa next r = nfa')
 
 theorem pathIn_of_compile_matches (eq : compile r = nfa)
   (m : r.matches cs) :
-  pathIn' nfa 1 nfa.start.val 0 cs := by
+  pathIn nfa 1 nfa.start.val 0 cs := by
   unfold NFA.compile at eq
   set result := NFA.done.pushRegex ⟨0, by decide⟩ r with h
   have := pathIn_of_matches h.symm m
