RegexCorrectness/VM/Correctness.lean
@@ -12,7 +12,7 @@ theorem matches_of_captureNext
   ∃ (s : Substring) (l m r : List Char),
     s.ValidFor l m r ∧ it.toString = ⟨l ++ m ++ r⟩ ∧ re.matches m := by
   have ⟨s, l, m, r, sv, eqs, i, hr, hdone⟩ := captureNext_spec h v hsome
-  have ma := matches_of_reaches' eq hr hdone
+  have ma := matches_of_reaches eq hr hdone
   exact ⟨s, l, m, r, sv, eqs, ma⟩
 
 end Regex.VM
